use dafny's new const feature in place of functions with no arguments
it's unclear if this improves verification performance directly, but
it does clean up the code a bit. non-trivial changes include:

 * additional calls to extractPageDbToAbstract lemma; seems like we're
   no longer triggering on constants like we were on the old functions

 * simplification/refactoring in the enter/resume paths, to avoid
   timeouts (it's unclear to me whether this is due to the const
   change, or recent work for SHA made this worse for some reason)

'make verified' passes; 'make verified/sha/sha256-refined.verified'
fails with the following timeouts:
  Impl$$_module.__default.sp__refined__Body__00__15
  Impl$$_module.__default.sp__refined__Body__16__XX

verified/ARMdef.dfy
@@ -7,13 +7,15 @@ include "words_and_bytes.s.dfy"
 //-----------------------------------------------------------------------------
 // Core types (for a 32-bit word-aligned machine)
 //-----------------------------------------------------------------------------
-//predicate isUInt32(i:int) { 0 <= i < 0x1_0000_0000 }
-function  BytesPerWord() : int { 4 }
-predicate WordAligned(i:int) { i % 4 == 0 }
-function  WordsToBytes(w:int) : int { 4 * w }
-function  BytesToWords(b:int) : int requires WordAligned(b) { b / 4 }
+const WORDSIZE:int := 4;
+predicate WordAligned(i:int) { i % WORDSIZE == 0 }
+function  WordsToBytes(w:int): int
+    ensures WordAligned(WordsToBytes(w))
+{ WORDSIZE * w }
+function  BytesToWords(b:int): int
+    requires WordAligned(b)
+{ b / WORDSIZE }
 
-//type word = x | isUInt32(x)
 type addr = x | isUInt32(x) && WordAligned(x)
 type shift_amount = s | 0 <= s < 32 // Some shifts allow s=32, but we'll be conservative for simplicity
 
@@ -362,8 +364,8 @@ predicate ValidMem(addr:int)
 
 predicate ValidMemRange(base:int, limit:int)
 {
-    isUInt32(base) && isUInt32(limit) &&
-    forall m:addr :: base <= m < limit && WordAligned(m) ==> m in TheValidAddresses()
+    ValidMem(base) && ValidMem(limit - WORDSIZE)
+    && forall a:addr :: base <= a < limit && WordAligned(a) ==> ValidMem(a)
 }
 
 predicate ValidShiftOperand(s:state, o:operand)
@@ -486,7 +488,7 @@ predicate evalEnterUserspace(s:state, r:state)
     evalUpdate(s, OSReg(cpsr), OperandContents(s, spsr), r)
 }
 
-predicate evalUserspaceExecution(s:state, r:state)
+predicate {:opaque} evalUserspaceExecution(s:state, r:state)
     requires ValidState(s)
     ensures  evalUserspaceExecution(s, r) ==>
         ValidState(r) && mode_of_state(r) == User;
@@ -524,13 +526,13 @@ predicate {:axiom} ApplicationUsermodeContinuationInvariant(s:state, r:state)
 // Model of page tables for userspace execution
 //-----------------------------------------------------------------------------
 
-function method PAGESIZE():int { 0x1000 }
+const PAGESIZE:int := 0x1000;
 
 predicate PageAligned(addr:int)
     ensures PageAligned(addr) ==> WordAligned(addr)
 {
     lemma_PageAlignedImpliesWordAligned(addr);
-    addr % PAGESIZE() == 0
+    addr % PAGESIZE == 0
 }
 
 // We model a trivial memory map (for our own code and page tables)
@@ -544,24 +546,20 @@ type AbsPTable = seq<Maybe<AbsL2PTable>>
 type AbsL2PTable = seq<Maybe<AbsPTE>>
 datatype AbsPTE = AbsPTE(phys: addr, write: bool, exec: bool)
 
-function method ARM_L1PTES(): int { 1024 }
-function method ARM_L1PTABLE_BYTES(): int
-    ensures ARM_L1PTABLE_BYTES() == WordsToBytes(ARM_L1PTES())
-{ 0x1000 }
-function method ARM_L2PTES(): int { 256 }
-function method ARM_L2PTABLE_BYTES(): int
-    ensures ARM_L2PTABLE_BYTES() == WordsToBytes(ARM_L2PTES())
-{ 0x400 }
+const ARM_L1PTES:int := 1024;
+const ARM_L1PTABLE_BYTES:int := PAGESIZE; // WordsToBytes(ARM_L1PTES)
+const ARM_L2PTES:int := 256;
+const ARM_L2PTABLE_BYTES:int := 0x400; // WordsToBytes(ARM_L2PTES)
 
 predicate WellformedAbsPTable(pt: AbsPTable)
 {
-    |pt| == ARM_L1PTES()
+    |pt| == ARM_L1PTES
         && forall i :: 0 <= i < |pt| && pt[i].Just? ==> WellformedAbsL2PTable(fromJust(pt[i]))
 }
 
 predicate WellformedAbsL2PTable(pt: AbsL2PTable)
 {
-    |pt| == ARM_L2PTES() && forall i :: 0 <= i < |pt| ==> WellformedAbsPTE(pt[i])
+    |pt| == ARM_L2PTES && forall i :: 0 <= i < |pt| ==> WellformedAbsPTE(pt[i])
 }
 
 predicate WellformedAbsPTE(pte: Maybe<AbsPTE>)
@@ -591,13 +589,18 @@ function WritablePagesInTable(pt:AbsPTable): set<addr>
           pt[i].v[j].v.phys + PhysBase()))
 }
 
+function WordOffset(a:addr, i:int): addr
+    requires isUInt32(a + WordsToBytes(i))
+    ensures WordAligned(WordOffset(a, i))
+{ a + WordsToBytes(i) }
+
 predicate ValidAbsL1PTable(m:memstate, vbase:int)
     requires ValidMemState(m)
 {
-    WordAligned(vbase) && ValidMemRange(vbase, vbase + ARM_L1PTABLE_BYTES())
+    WordAligned(vbase) && ValidMemRange(vbase, vbase + ARM_L1PTABLE_BYTES)
     // all L1 PTEs are valid, and all non-zero PTEs point to valid L2 tables
-    && forall i | 0 <= i < ARM_L1PTES() :: (
-        var ptew := MemContents(m, vbase + WordsToBytes(i));
+    && forall i | 0 <= i < ARM_L1PTES :: (
+        var ptew := MemContents(m, WordOffset(vbase, i));
         ValidAbsL1PTEWord(ptew) &&
             var ptem := ExtractAbsL1PTE(ptew);
             ptem.Just? ==> (
@@ -610,11 +613,11 @@ function ExtractAbsL1PTable(m:memstate, vbase:addr): AbsPTable
     requires ValidAbsL1PTable(m, vbase)
     ensures WellformedAbsPTable(ExtractAbsL1PTable(m, vbase))
 {
-    var f := imap i | 0 <= i < ARM_L1PTES() :: (
-        var pte := ExtractAbsL1PTE(MemContents(m, vbase + WordsToBytes(i)));
+    var f := imap i | 0 <= i < ARM_L1PTES :: (
+        var pte := ExtractAbsL1PTE(MemContents(m, WordOffset(vbase, i)));
         if pte.Nothing? then Nothing else Just(ExtractAbsL2PTable(m, pte.v + PhysBase()))
         );
-    var indices := SeqOfNumbersInRightExclusiveRange(0, ARM_L1PTES());
+    var indices := SeqOfNumbersInRightExclusiveRange(0, ARM_L1PTES);
     IMapSeqToSeq(indices, f)
 }
 
@@ -645,8 +648,8 @@ predicate ValidAbsL2PTable(m:memstate, vbase:addr)
     requires ValidMemState(m)
 {
     WordAligned(vbase)
-        && ValidMemRange(vbase, vbase + ARM_L2PTABLE_BYTES())
-        && forall i | 0 <= i < ARM_L2PTES() :: ValidAbsL2PTEWord(MemContents(m, vbase + WordsToBytes(i)))
+        && ValidMemRange(vbase, vbase + ARM_L2PTABLE_BYTES)
+        && forall i | 0 <= i < ARM_L2PTES :: ValidAbsL2PTEWord(MemContents(m, WordOffset(vbase, i)))
 }
 
 function ExtractAbsL2PTable(m:memstate, vbase:addr): AbsL2PTable
@@ -654,20 +657,14 @@ function ExtractAbsL2PTable(m:memstate, vbase:addr): AbsL2PTable
     requires ValidAbsL2PTable(m, vbase)
     ensures WellformedAbsL2PTable(ExtractAbsL2PTable(m, vbase))
 {
-    var f := imap i | 0 <= i < ARM_L2PTES() :: ExtractAbsL2PTE(MemContents(m, vbase + WordsToBytes(i)));
-    var indices := SeqOfNumbersInRightExclusiveRange(0, ARM_L2PTES());
+    var f := imap i | 0 <= i < ARM_L2PTES :: ExtractAbsL2PTE(MemContents(m, WordOffset(vbase, i)));
+    var indices := SeqOfNumbersInRightExclusiveRange(0, ARM_L2PTES);
     IMapSeqToSeq(indices, f)
 }
 
-function method ARM_L2PTE_NX_BIT(): bv32
-{
-    0x1 // XN
-}
-
-function method ARM_L2PTE_RO_BIT(): bv32
-{
-    0x200 // AP2
-}
+const ARM_L2PTE_NX_BIT: bv32 := 0x1; // XN
+const ARM_L2PTE_RO_BIT: bv32 := 0x200; // AP2
+const ARM_L2PTE_CONST_BITS: bv32 := 0xd74; // B, AP0, AP1, TEX, S, NG
 
 predicate ValidAbsL2PTEWord(pteword:word)
 {
@@ -675,7 +672,7 @@ predicate ValidAbsL2PTEWord(pteword:word)
     var typebits := BitAnd(pte, 0x3);
     var lowbits := BitAnd(pte, 0xdfc);
     var pagebase := BitwiseMaskHigh(pteword, 12);
-    typebits == 0 || (typebits != 1 && lowbits == ARM_L2PTE_CONST_BITS() && isUInt32(pagebase + PhysBase()))
+    typebits == 0 || (typebits != 1 && lowbits == ARM_L2PTE_CONST_BITS && isUInt32(pagebase + PhysBase()))
 }
 
 function ExtractAbsL2PTE(pteword:word): Maybe<AbsPTE>
@@ -684,21 +681,12 @@ function ExtractAbsL2PTE(pteword:word): Maybe<AbsPTE>
 {
     var pte := WordAsBits(pteword);
     var typebits := BitAnd(pte, 0x3);
-    var exec := BitAnd(pte, ARM_L2PTE_NX_BIT()) == 0;
-    var write := BitAnd(pte, ARM_L2PTE_RO_BIT()) == 0;
+    var exec := BitAnd(pte, ARM_L2PTE_NX_BIT) == 0;
+    var write := BitAnd(pte, ARM_L2PTE_RO_BIT) == 0;
     var pagebase := BitwiseMaskHigh(pteword, 12); // BitwiseAnd(pteword, 0xfffff000);
     assert PageAligned(pagebase);
     // if the type is zero, it's an invalid entry, which is fine (maps nothing)
     if typebits == 0 then Nothing else Just(AbsPTE(pagebase, write, exec))
-}
-
-function method ARM_L2PTE_CONST_BITS(): bv32
-{
-    0x4 /* B */
-        | 0x30 /* AP0, AP1 */
-        | 0x140 /* TEX */
-        | 0x400 /* S */
-        | 0x800 /* NG */
 }
 
 //-----------------------------------------------------------------------------
