verified/kom_common.s.dfy
@@ -1,92 +1,84 @@
 include "ARMdef.dfy"
 
-function method KOM_MAGIC():int { 0x4b6d646f }
+const KOM_MAGIC:int := 0x4b6d646f;
 
 //-----------------------------------------------------------------------------
 // SMC Call Numbers
 //-----------------------------------------------------------------------------
-function method KOM_SMC_QUERY():int           { 1  }
-function method KOM_SMC_GETPHYSPAGES():int    { 2  }
-function method KOM_SMC_INIT_ADDRSPACE():int  { 10 }
-function method KOM_SMC_INIT_DISPATCHER():int { 11 }
-function method KOM_SMC_INIT_L2PTABLE():int   { 12 }
-function method KOM_SMC_MAP_SECURE():int      { 13 }
-function method KOM_SMC_MAP_INSECURE():int    { 14 }
-function method KOM_SMC_REMOVE():int          { 20 }
-function method KOM_SMC_FINALISE():int        { 21 }
-function method KOM_SMC_ENTER():int           { 22 }
-function method KOM_SMC_RESUME():int          { 23 }
-function method KOM_SMC_STOP():int            { 29 }
+const KOM_SMC_QUERY:int             := 1;
+const KOM_SMC_GETPHYSPAGES:int      := 2;
+const KOM_SMC_INIT_ADDRSPACE:int    := 10;
+const KOM_SMC_INIT_DISPATCHER:int   := 11;
+const KOM_SMC_INIT_L2PTABLE:int     := 12;
+const KOM_SMC_MAP_SECURE:int        := 13;
+const KOM_SMC_MAP_INSECURE:int      := 14;
+const KOM_SMC_REMOVE:int            := 20;
+const KOM_SMC_FINALISE:int          := 21;
+const KOM_SMC_ENTER:int             := 22;
+const KOM_SMC_RESUME:int            := 23;
+const KOM_SMC_STOP:int              := 29;
 
 //-----------------------------------------------------------------------------
 // Errors
 //-----------------------------------------------------------------------------
-function method KOM_ERR_SUCCESS():int            { 0  }
-function method KOM_ERR_INVALID_PAGENO():int     { 1  }
-function method KOM_ERR_PAGEINUSE():int          { 2  }
-function method KOM_ERR_INVALID_ADDRSPACE():int  { 3  }
-function method KOM_ERR_ALREADY_FINAL():int      { 4  }
-function method KOM_ERR_NOT_FINAL():int          { 5  }
-function method KOM_ERR_INVALID_MAPPING():int    { 6  }
-function method KOM_ERR_ADDRINUSE():int          { 7  }
-function method KOM_ERR_NOT_STOPPED():int        { 8  }
-function method KOM_ERR_INTERRUPTED():int        { 9  }
-function method KOM_ERR_FAULT():int              { 10 }
-function method KOM_ERR_ALREADY_ENTERED():int    { 11 }
-function method KOM_ERR_NOT_ENTERED():int        { 12 }
-function method KOM_ERR_INVALID():int            { 0xffffffff }
+const KOM_ERR_SUCCESS:int           := 0;
+const KOM_ERR_INVALID_PAGENO:int    := 1;
+const KOM_ERR_PAGEINUSE:int         := 2;
+const KOM_ERR_INVALID_ADDRSPACE:int := 3;
+const KOM_ERR_ALREADY_FINAL:int     := 4;
+const KOM_ERR_NOT_FINAL:int         := 5;
+const KOM_ERR_INVALID_MAPPING:int   := 6;
+const KOM_ERR_ADDRINUSE:int         := 7;
+const KOM_ERR_NOT_STOPPED:int       := 8;
+const KOM_ERR_INTERRUPTED:int       := 9;
+const KOM_ERR_FAULT:int             := 10;
+const KOM_ERR_ALREADY_ENTERED:int   := 11;
+const KOM_ERR_NOT_ENTERED:int       := 12;
+const KOM_ERR_INVALID:int           := 0xffffffff;
 
 //-----------------------------------------------------------------------------
 // Memory Regions
 //-----------------------------------------------------------------------------
-function method KOM_MON_VBASE():addr
-    { 0x4000_0000 }
-function method KOM_DIRECTMAP_VBASE():addr
-    { 0x8000_0000 }
-function method KOM_DIRECTMAP_SIZE():word   { 0x8000_0000 }
-function method KOM_SECURE_RESERVE():addr
-    { 1 * 1024 * 1024 }
-function method KOM_SECURE_NPAGES():word
-    ensures KOM_SECURE_NPAGES() == 256;
-    { KOM_SECURE_RESERVE() / PAGESIZE() }
+const KOM_MON_VBASE:addr := 0x4000_0000;
+const KOM_DIRECTMAP_VBASE:addr := 0x8000_0000;
+const KOM_DIRECTMAP_SIZE:word := 0x8000_0000;
+const KOM_SECURE_RESERVE:addr := 0x100000; // 1MB
+const KOM_SECURE_NPAGES:word := 256; // KOM_SECURE_RESERVE / PAGESIZE
 
 // we don't support/consider more than 1GB of physical memory in our maps
-function method KOM_PHYSMEM_LIMIT():addr
-    { 0x4000_0000 }
+const KOM_PHYSMEM_LIMIT:addr := 0x4000_0000;
 
-function KOM_STACK_SIZE():addr
-    { 0x4000 }
+const KOM_STACK_SIZE:addr := 0x4000;
 
 // we don't know where the stack is exactly, but we know how big it is
 function {:axiom} StackLimit():addr
-    ensures KOM_MON_VBASE() <= StackLimit()
-    ensures StackLimit() <= KOM_DIRECTMAP_VBASE() - KOM_STACK_SIZE()
+    ensures KOM_MON_VBASE <= StackLimit()
+    ensures StackLimit() <= KOM_DIRECTMAP_VBASE - KOM_STACK_SIZE
 
 function StackBase():addr
 {
-    StackLimit() + KOM_STACK_SIZE()
+    StackLimit() + KOM_STACK_SIZE
 }
 
 predicate address_is_secure(m:addr)
 {
-    (KOM_DIRECTMAP_VBASE() + SecurePhysBase()) <= m <
-        (KOM_DIRECTMAP_VBASE() + SecurePhysBase() + KOM_SECURE_RESERVE())
+    (KOM_DIRECTMAP_VBASE + SecurePhysBase()) <= m <
+        (KOM_DIRECTMAP_VBASE + SecurePhysBase() + KOM_SECURE_RESERVE)
 }
 
 //-----------------------------------------------------------------------------
 //  Memory Mapping Config Args
 //-----------------------------------------------------------------------------
-function method KOM_MAPPING_R():int     { 1 }
-function method KOM_MAPPING_W():int     { 2 }
-function method KOM_MAPPING_X():int     { 4 }
+const KOM_MAPPING_R:int := 1;
+const KOM_MAPPING_W:int := 2;
+const KOM_MAPPING_X:int := 4;
 
 //-----------------------------------------------------------------------------
 // Globals
 //-----------------------------------------------------------------------------
 
-function method PAGEDB_ENTRY_SIZE():int { 8 }
-function method G_PAGEDB_SIZE():int
-    { KOM_SECURE_NPAGES() * PAGEDB_ENTRY_SIZE() }
+const PAGEDB_ENTRY_SIZE:int := 8;
+const G_PAGEDB_SIZE:int := KOM_SECURE_NPAGES * PAGEDB_ENTRY_SIZE;
 
 function method {:opaque} PageDb(): symbol { "g_pagedb" }
 function method {:opaque} SecurePhysBaseOp(): symbol {"g_secure_physbase" }
@@ -95,15 +87,15 @@ function method {:opaque} K_SHA256s(): symbol { "g_k_sha256" }
 
 // the phys base is unknown, but never changes
 function method {:axiom} SecurePhysBase(): addr
-    ensures 0 < SecurePhysBase() <= KOM_PHYSMEM_LIMIT() - KOM_SECURE_RESERVE();
+    ensures 0 < SecurePhysBase() <= KOM_PHYSMEM_LIMIT - KOM_SECURE_RESERVE;
     ensures PageAligned(SecurePhysBase());
 
 function method KomGlobalDecls(): globaldecls
     ensures ValidGlobalDecls(KomGlobalDecls());
 {
-    map[SecurePhysBaseOp() := 4, //BytesPerWord() 
-        CurDispatcherOp() := 4,   //BytesPerWord()
-        PageDb() := G_PAGEDB_SIZE(),
+    map[SecurePhysBaseOp() := WORDSIZE,
+        CurDispatcherOp() := WORDSIZE,
+        PageDb() := G_PAGEDB_SIZE,
         K_SHA256s() := 256
         ]
 }
@@ -132,11 +124,11 @@ predicate SaneMem(s:memstate)
 
 predicate SaneConstants()
 {
-    PhysBase() == KOM_DIRECTMAP_VBASE()
+    PhysBase() == KOM_DIRECTMAP_VBASE
     && TheValidAddresses() == (
         // our secure phys mapping must be valid
-        (set m:addr | KOM_DIRECTMAP_VBASE() + SecurePhysBase() <= m
-               < KOM_DIRECTMAP_VBASE() + SecurePhysBase() + KOM_SECURE_RESERVE())
+        (set m:addr | KOM_DIRECTMAP_VBASE + SecurePhysBase() <= m
+               < KOM_DIRECTMAP_VBASE + SecurePhysBase() + KOM_SECURE_RESERVE)
         // the stack must be mapped
         + (set m:addr | StackLimit() <= m < StackBase()))
     // TODO: our insecure phys mapping must be valid
