verified/smcapi.s.dfy
@@ -11,7 +11,7 @@ predicate l1indexInUse(d: PageDb, a: PageNr, l1index: int)
     requires validPageDb(d)
     requires isAddrspace(d, a)
     requires !stoppedAddrspace(d[a])
-    requires 0 <= l1index < NR_L1PTES()
+    requires 0 <= l1index < NR_L1PTES
 {
     reveal_validPageDb();
     assert validAddrspace(d, a);
@@ -25,7 +25,7 @@ function updateL2Pte(d: PageDb, a: PageNr, mapping: Mapping, l2e : L2PTE)
     requires validPageDb(d)
     requires isAddrspace(d, a)
     requires validMapping(mapping,d,a)
-    //requires isValidMappingTarget(d, a, mapping) == KOM_ERR_SUCCESS()
+    //requires isValidMappingTarget(d, a, mapping) == KOM_ERR_SUCCESS
     requires d[a].entry.state.InitState?
     requires validL2PTE(d, a, l2e)
 {
@@ -43,7 +43,7 @@ function isValidMappingTarget(d: PageDb, a: PageNr, mapping: word)
     : int // KOM_ERROR
     requires validPageDb(d)
     requires isAddrspace(d, a)
-    ensures  isValidMappingTarget(d,a,mapping) == KOM_ERR_SUCCESS() ==>
+    ensures  isValidMappingTarget(d,a,mapping) == KOM_ERR_SUCCESS ==>
         validMapping(wordToMapping(mapping),d,a)
 {
     reveal_validPageDb();
@@ -53,29 +53,29 @@ function isValidMappingTarget(d: PageDb, a: PageNr, mapping: word)
     var l2index := l2indexFromMapping(mapping);
     var perm := permFromMapping(mapping);
     if(!addrspace.state.InitState?) then
-        KOM_ERR_ALREADY_FINAL()
+        KOM_ERR_ALREADY_FINAL
     else if(!validPageNr(l1indexFromMapping(mapping)) ||
         !validPageNr(l2indexFromMapping(mapping))) then
-        KOM_ERR_INVALID_MAPPING()
+        KOM_ERR_INVALID_MAPPING
     else 
-        if(!perm.r) then KOM_ERR_INVALID_MAPPING()
-        else if(!(0 <= l1index < NR_L1PTES())
-            || !(0 <= l2index < NR_L2PTES()) ) then
-            KOM_ERR_INVALID_MAPPING()
+        if(!perm.r) then KOM_ERR_INVALID_MAPPING
+        else if(!(0 <= l1index < NR_L1PTES)
+            || !(0 <= l2index < NR_L2PTES) ) then
+            KOM_ERR_INVALID_MAPPING
         else
             assert validAddrspace(d, a);
             var l1 := d[addrspace.l1ptnr].entry;
             var l1pte := l1.l1pt[l1index];
-            if(l1pte.Nothing?) then KOM_ERR_INVALID_MAPPING()
-            else KOM_ERR_SUCCESS()
+            if(l1pte.Nothing?) then KOM_ERR_INVALID_MAPPING
+            else KOM_ERR_SUCCESS
 }
 
 //============================================================================
 // Behavioral Specification of Monitor Calls
 //=============================================================================
-function smc_query() : int { KOM_MAGIC() }
+function smc_query() : int { KOM_MAGIC }
 
-function smc_getPhysPages() : int { KOM_SECURE_NPAGES() }
+function smc_getPhysPages() : int { KOM_SECURE_NPAGES }
 
 function smc_initAddrspace(pageDbIn: PageDb, addrspacePage: word, l1PTPage: word)
     : (PageDb, word) // PageDbOut, KOM_ERR
@@ -85,18 +85,18 @@ function smc_initAddrspace(pageDbIn: PageDb, addrspacePage: word, l1PTPage: word
     var g := pageDbIn;
     if(!validPageNr(addrspacePage) || !validPageNr(l1PTPage) ||
         addrspacePage == l1PTPage) then
-        (pageDbIn, KOM_ERR_INVALID_PAGENO())
+        (pageDbIn, KOM_ERR_INVALID_PAGENO)
     else if(l1PTPage % 4 != 0) then
-        (pageDbIn, KOM_ERR_INVALID_PAGENO())
+        (pageDbIn, KOM_ERR_INVALID_PAGENO)
     else if( !g[addrspacePage].PageDbEntryFree? || !g[l1PTPage].PageDbEntryFree? ) then
-        (pageDbIn, KOM_ERR_PAGEINUSE())
+        (pageDbIn, KOM_ERR_PAGEINUSE)
     else
         var addrspace := Addrspace(l1PTPage, 1, InitState);
-        var l1PT := L1PTable(SeqRepeat(NR_L1PTES(),Nothing));
+        var l1PT := L1PTable(SeqRepeat(NR_L1PTES,Nothing));
         var pageDbOut := 
             (pageDbIn[addrspacePage := PageDbEntryTyped(addrspacePage, addrspace)])[
                 l1PTPage := PageDbEntryTyped(addrspacePage, l1PT)];
-        (pageDbOut, KOM_ERR_SUCCESS())
+        (pageDbOut, KOM_ERR_SUCCESS)
 }
 
 function initDispCtxt() : DispatcherContext
@@ -123,14 +123,14 @@ function smc_initDispatcher(pageDbIn: PageDb, page:word, addrspacePage:word,
 {
     reveal_validPageDb();
     if(!isAddrspace(pageDbIn, addrspacePage)) then
-        (pageDbIn, KOM_ERR_INVALID_ADDRSPACE())
+        (pageDbIn, KOM_ERR_INVALID_ADDRSPACE)
     else
         allocatePage(pageDbIn, page, addrspacePage, Dispatcher(entrypoint, false, initDispCtxt()))
 }
 
 function installL1PTE(l1pt: PageDbEntryTyped, l2page: PageNr, l1index: int): PageDbEntryTyped
     requires l1pt.L1PTable? && wellFormedPageDbEntryTyped(l1pt)
-    requires 0 <= l1index < NR_L1PTES()
+    requires 0 <= l1index < NR_L1PTES
     ensures var r := installL1PTE(l1pt, l2page, l1index);
         r.L1PTable? && wellFormedPageDbEntryTyped(r)
 {
@@ -141,7 +141,7 @@ function installL1PTEInPageDb(pagedb: PageDb, l1ptnr: PageNr, l2page: PageNr,
     l1index: int): PageDb
     requires validPageDb(pagedb)
     requires pagedb[l1ptnr].PageDbEntryTyped? && pagedb[l1ptnr].entry.L1PTable?
-    requires 0 <= l1index < NR_L1PTES()
+    requires 0 <= l1index < NR_L1PTES
     ensures wellFormedPageDb(installL1PTEInPageDb(pagedb, l1ptnr, l2page, l1index))
 {
     reveal_validPageDb();
@@ -154,9 +154,9 @@ function smc_initL2PTable(pageDbIn: PageDb, page: word, addrspacePage: word,
     requires validPageDb(pageDbIn)
 {
     reveal_validPageDb();
-    if(!(0<= l1index < NR_L1PTES())) then (pageDbIn, KOM_ERR_INVALID_MAPPING())
+    if(!(0<= l1index < NR_L1PTES)) then (pageDbIn, KOM_ERR_INVALID_MAPPING)
     else if(!isAddrspace(pageDbIn, addrspacePage)) then
-        (pageDbIn, KOM_ERR_INVALID_ADDRSPACE())
+        (pageDbIn, KOM_ERR_INVALID_ADDRSPACE)
 
     // This gets caught later in allocatePage, but putting the check
     // here means that the addrspace's state will not be stopped for the
@@ -164,15 +164,15 @@ function smc_initL2PTable(pageDbIn: PageDb, page: word, addrspacePage: word,
     // is actually an l1pt table, which is true as long as the addrspace
     // is not stopped.
     else if(pageDbIn[addrspacePage].entry.state != InitState) then
-        (pageDbIn, KOM_ERR_ALREADY_FINAL())
+        (pageDbIn, KOM_ERR_ALREADY_FINAL)
     else if(l1indexInUse(pageDbIn, addrspacePage, l1index)) then
-        (pageDbIn, KOM_ERR_ADDRINUSE())
+        (pageDbIn, KOM_ERR_ADDRINUSE)
     else 
-        var l2pt := L2PTable(SeqRepeat(NR_L2PTES(), NoMapping));
+        var l2pt := L2PTable(SeqRepeat(NR_L2PTES, NoMapping));
         // allocate the page
         var (pagedb, err) := allocatePage(pageDbIn, page, addrspacePage, l2pt);
         // update the L1 table
-        if err == KOM_ERR_SUCCESS() then
+        if err == KOM_ERR_SUCCESS then
             var l1ptnr := pagedb[addrspacePage].entry.l1ptnr;
             (installL1PTEInPageDb(pagedb, l1ptnr, page, l1index), err)
         else
@@ -183,7 +183,7 @@ predicate allocatePageEntryValid(entry: PageDbEntryTyped)
 {
     wellFormedPageDbEntryTyped(entry)
     && ((entry.Dispatcher? && !entry.entered)
-        || (entry.L2PTable? && entry.l2pt == SeqRepeat(NR_L2PTES(), NoMapping))
+        || (entry.L2PTable? && entry.l2pt == SeqRepeat(NR_L2PTES, NoMapping))
         || entry.DataPage?)
 }
 
@@ -197,17 +197,17 @@ function allocatePage_inner(pageDbIn: PageDb, securePage: word,
 {
     reveal_validPageDb();
     var addrspace := pageDbIn[addrspacePage].entry;
-    if(!validPageNr(securePage)) then (pageDbIn, KOM_ERR_INVALID_PAGENO())
-    else if(!pageIsFree(pageDbIn, securePage)) then (pageDbIn, KOM_ERR_PAGEINUSE())
+    if(!validPageNr(securePage)) then (pageDbIn, KOM_ERR_INVALID_PAGENO)
+    else if(!pageIsFree(pageDbIn, securePage)) then (pageDbIn, KOM_ERR_PAGEINUSE)
     else if(addrspace.state != InitState) then
-        (pageDbIn,KOM_ERR_ALREADY_FINAL())
+        (pageDbIn,KOM_ERR_ALREADY_FINAL)
     // TODO ?? Model page clearing for non-data pages?
     else
         var updatedAddrspace := addrspace.(refcount := addrspace.refcount + 1);
         var pageDbOut := (pageDbIn[
             securePage := PageDbEntryTyped(addrspacePage, entry)])[
             addrspacePage := pageDbIn[addrspacePage].(entry := updatedAddrspace)];
-        (pageDbOut, KOM_ERR_SUCCESS())
+        (pageDbOut, KOM_ERR_SUCCESS)
 }
 
 // TODO move this elsewhere since it is not a monitor call
@@ -219,7 +219,7 @@ function allocatePage(pageDbIn: PageDb, securePage: word,
     requires allocatePageEntryValid(entry)
     ensures  validPageDb(allocatePage(pageDbIn, securePage, addrspacePage, entry).0);
     ensures  allocatePage(pageDbIn, securePage, addrspacePage, entry).1 == 
-        KOM_ERR_SUCCESS() ==> validPageNr(securePage);
+        KOM_ERR_SUCCESS ==> validPageNr(securePage);
 {
     reveal_validPageDb();
     allocatePagePreservesPageDBValidity(pageDbIn, securePage, addrspacePage, entry);
@@ -233,26 +233,26 @@ function smc_remove(pageDbIn: PageDb, page: word)
 {
     reveal_validPageDb();
     if(!validPageNr(page)) then
-        (pageDbIn, KOM_ERR_INVALID_PAGENO())
+        (pageDbIn, KOM_ERR_INVALID_PAGENO)
     else if(pageDbIn[page].PageDbEntryFree?) then
-        (pageDbIn, KOM_ERR_SUCCESS())
+        (pageDbIn, KOM_ERR_SUCCESS)
     else 
         var e := pageDbIn[page].entry;
         var addrspacePage := pageDbIn[page].addrspace;
         var addrspace := pageDbIn[addrspacePage].entry;
         if( e.Addrspace? ) then
-           if(e.refcount !=0) then (pageDbIn, KOM_ERR_PAGEINUSE())
-           else (pageDbIn[page := PageDbEntryFree], KOM_ERR_SUCCESS())
+           if(e.refcount !=0) then (pageDbIn, KOM_ERR_PAGEINUSE)
+           else (pageDbIn[page := PageDbEntryFree], KOM_ERR_SUCCESS)
         else 
             if( !addrspace.state.StoppedState?) then
-                (pageDbIn, KOM_ERR_NOT_STOPPED())
+                (pageDbIn, KOM_ERR_NOT_STOPPED)
             else 
                 var d := pageDbIn; var p := page; var a := addrspacePage;
                 assert p in addrspaceRefs(d, a);
                 var d' := (d[p := PageDbEntryFree])
                         [a := d[a].( entry := d[a].entry.( refcount := 
                             d[a].entry.refcount - 1 ))];
-                (d', KOM_ERR_SUCCESS())
+                (d', KOM_ERR_SUCCESS)
 }
 
 function smc_mapSecure(pageDbIn: PageDb, page: word, addrspacePage: word,
@@ -261,26 +261,26 @@ function smc_mapSecure(pageDbIn: PageDb, page: word, addrspacePage: word,
 {
     reveal_validPageDb();
     if(!isAddrspace(pageDbIn, addrspacePage)) then
-        (pageDbIn, KOM_ERR_INVALID_ADDRSPACE())
+        (pageDbIn, KOM_ERR_INVALID_ADDRSPACE)
     else 
         var err := isValidMappingTarget(pageDbIn, addrspacePage, mapping);
-        if( err != KOM_ERR_SUCCESS() ) then (pageDbIn, err)
+        if( err != KOM_ERR_SUCCESS ) then (pageDbIn, err)
         else 
             var abs_mapping := wordToMapping(mapping);
             // Check physPage (which is optionally used to populate
             // the initial contents of the secure page) for validity
             if (physPage != 0 && !physPageIsInsecureRam(physPage)) then
-                (pageDbIn, KOM_ERR_INVALID_PAGENO())
+                (pageDbIn, KOM_ERR_INVALID_PAGENO)
             else
                 var ap_ret := allocatePage(pageDbIn, page,
                     addrspacePage, DataPage);
                 var pageDbA := ap_ret.0;
                 var errA := ap_ret.1;
-                if(errA != KOM_ERR_SUCCESS()) then (pageDbIn, errA)
+                if(errA != KOM_ERR_SUCCESS) then (pageDbIn, errA)
                 else
                     var l2pte := SecureMapping(page, abs_mapping.perm.w, abs_mapping.perm.x);
                     var pageDbOut := updateL2Pte(pageDbA, addrspacePage, abs_mapping, l2pte);
-                    (pageDbOut, KOM_ERR_SUCCESS())
+                    (pageDbOut, KOM_ERR_SUCCESS)
 }
 
 function smc_mapInsecure(pageDbIn: PageDb, addrspacePage: word,
@@ -289,18 +289,18 @@ function smc_mapInsecure(pageDbIn: PageDb, addrspacePage: word,
 {
     reveal_validPageDb();
     if(!isAddrspace(pageDbIn, addrspacePage)) then
-        (pageDbIn, KOM_ERR_INVALID_ADDRSPACE())
+        (pageDbIn, KOM_ERR_INVALID_ADDRSPACE)
     else
         var err := isValidMappingTarget(pageDbIn, addrspacePage, mapping);
-        if( err != KOM_ERR_SUCCESS() ) then (pageDbIn, err)
+        if( err != KOM_ERR_SUCCESS ) then (pageDbIn, err)
         else if(!physPageIsInsecureRam(physPage)) then
-            (pageDbIn, KOM_ERR_INVALID_PAGENO())
+            (pageDbIn, KOM_ERR_INVALID_PAGENO)
         else
             var abs_mapping := wordToMapping(mapping);
             assert validInsecurePageNr(physPage);
             var l2pte := InsecureMapping( physPage,  abs_mapping.perm.w);
             var pageDbOut := updateL2Pte(pageDbIn, addrspacePage, abs_mapping, l2pte);
-            (pageDbOut, KOM_ERR_SUCCESS())
+            (pageDbOut, KOM_ERR_SUCCESS)
 }
 
 function smc_finalise(pageDbIn: PageDb, addrspacePage: word) : (PageDb, word)
@@ -309,12 +309,12 @@ function smc_finalise(pageDbIn: PageDb, addrspacePage: word) : (PageDb, word)
     reveal_validPageDb();
     var d := pageDbIn; var a := addrspacePage;
     if(!isAddrspace(pageDbIn, addrspacePage)) then
-        (pageDbIn, KOM_ERR_INVALID_ADDRSPACE())
+        (pageDbIn, KOM_ERR_INVALID_ADDRSPACE)
     else if(pageDbIn[addrspacePage].entry.state != InitState) then
-        (pageDbIn, KOM_ERR_ALREADY_FINAL())
+        (pageDbIn, KOM_ERR_ALREADY_FINAL)
     else
         var d' := d[ a := d[a].( entry := d[a].entry.( state := FinalState ))];
-        (d', KOM_ERR_SUCCESS())
+        (d', KOM_ERR_SUCCESS)
 }
 
 function smc_stop(pageDbIn: PageDb, addrspacePage: word)
@@ -324,10 +324,10 @@ function smc_stop(pageDbIn: PageDb, addrspacePage: word)
     reveal_validPageDb();
     var d := pageDbIn; var a := addrspacePage;
     if(!isAddrspace(pageDbIn, addrspacePage)) then
-        (pageDbIn, KOM_ERR_INVALID_ADDRSPACE())
+        (pageDbIn, KOM_ERR_INVALID_ADDRSPACE)
     else
         var d' := d[ a := d[a].( entry := d[a].entry.( state := StoppedState ))];
-        (d', KOM_ERR_SUCCESS())
+        (d', KOM_ERR_SUCCESS)
 }
 
 //=============================================================================
@@ -341,32 +341,32 @@ predicate smchandler(s: state, pageDbIn: PageDb, s':state, pageDbOut: PageDb)
         := s.regs[R0], s.regs[R1], s.regs[R2], s.regs[R3], s.regs[R4];
     var err, val := s'.regs[R0], s'.regs[R1];
 
-    if callno == KOM_SMC_QUERY() then
-        pageDbOut == pageDbIn && err == KOM_MAGIC() && val == 0
-    else if callno == KOM_SMC_GETPHYSPAGES() then
-        pageDbOut == pageDbIn && err == KOM_ERR_SUCCESS() && val == KOM_SECURE_NPAGES()
-    else if callno == KOM_SMC_INIT_ADDRSPACE() then
+    if callno == KOM_SMC_QUERY then
+        pageDbOut == pageDbIn && err == KOM_MAGIC && val == 0
+    else if callno == KOM_SMC_GETPHYSPAGES then
+        pageDbOut == pageDbIn && err == KOM_ERR_SUCCESS && val == KOM_SECURE_NPAGES
+    else if callno == KOM_SMC_INIT_ADDRSPACE then
         (pageDbOut, err) == smc_initAddrspace(pageDbIn, arg1, arg2) && val == 0
-    else if callno == KOM_SMC_INIT_DISPATCHER() then
+    else if callno == KOM_SMC_INIT_DISPATCHER then
         (pageDbOut, err) == smc_initDispatcher(pageDbIn, arg1, arg2, arg3) && val == 0
-    else if callno == KOM_SMC_INIT_L2PTABLE() then
+    else if callno == KOM_SMC_INIT_L2PTABLE then
         (pageDbOut, err) == smc_initL2PTable(pageDbIn, arg1, arg2, arg3) && val == 0
-    else if callno == KOM_SMC_MAP_SECURE() then
+    else if callno == KOM_SMC_MAP_SECURE then
         (pageDbOut, err) == smc_mapSecure(pageDbIn, arg1, arg2, arg3, arg4) && val == 0
-    else if callno == KOM_SMC_MAP_INSECURE() then
+    else if callno == KOM_SMC_MAP_INSECURE then
         (pageDbOut, err) == smc_mapInsecure(pageDbIn, arg1, arg2, arg3) && val == 0
-    else if callno == KOM_SMC_REMOVE() then
+    else if callno == KOM_SMC_REMOVE then
         (pageDbOut, err) == smc_remove(pageDbIn, arg1) && val == 0
-    else if callno == KOM_SMC_FINALISE() then
+    else if callno == KOM_SMC_FINALISE then
         (pageDbOut, err) == smc_finalise(pageDbIn, arg1) && val == 0
-    else if callno == KOM_SMC_ENTER() then
+    else if callno == KOM_SMC_ENTER then
         smc_enter(s, pageDbIn, s', pageDbOut, arg1, arg2, arg3, arg4)
-    else if callno == KOM_SMC_RESUME() then
+    else if callno == KOM_SMC_RESUME then
         smc_resume(s, pageDbIn, s', pageDbOut, arg1)
-    else if callno == KOM_SMC_STOP() then
+    else if callno == KOM_SMC_STOP then
         (pageDbOut, err) == smc_stop(pageDbIn, arg1) && val == 0
     else
-        pageDbOut == pageDbIn && err == KOM_ERR_INVALID() && val == 0)
+        pageDbOut == pageDbIn && err == KOM_ERR_INVALID && val == 0)
 }
 
 // non-volatile regs preserved
@@ -416,7 +416,7 @@ lemma allocatePagePreservesPageDBValidity(pageDbIn: PageDb,
     var pageDbOut := result.0;
     var errOut := result.1;
 
-    if ( errOut != KOM_ERR_SUCCESS() ){
+    if ( errOut != KOM_ERR_SUCCESS ){
         // The error case is trivial because PageDbOut == PageDbIn
     } else {
         forall () ensures validPageDbEntry(pageDbOut, addrspacePage);
